cleanup

Semantics/Stlc/Typing.lean
@@ -2,38 +2,40 @@ import Semantics.Stlc.Rewrite
 import Mathlib.Logic.Function.Basic
 
 def Context := String → Option Ty
-def empty_ctx: Context := λ _ ↦ none
+def Γ₀: Context := λ _ ↦ none
 
 inductive has_type: Context → Term → Ty → Prop where
   | var (h: Γ x = some T):
     has_type Γ (Term.var x) T
   | abs (h: has_type (Function.update Γ x (some T₂)) t T₁):
     has_type Γ (Λ x:T₂ ↦ t) (T₂ → T₁)
-  | app (h₁: has_type Γ t₁ (T₂ → T₁)) (h₂: has_type Γ t₂ T₂):
+  | app t₁ t₂
+    (h₁: has_type Γ t₁ (T₂ → T₁)) (h₂: has_type Γ t₂ T₂):
     has_type Γ (t₁..t₂) T₁
   | tt:
     has_type Γ ⊤ 𝔹
   | ff:
     has_type Γ ⊥ 𝔹
-  | cond (h₁: has_type Γ b 𝔹) (h₂: has_type Γ t₁ T₁) (h₃: has_type Γ t₂ T₁):
+  | cond t₁ t₂
+    (h₁: has_type Γ b 𝔹) (h₂: has_type Γ t₁ T₁) (h₃: has_type Γ t₂ T₁):
     has_type Γ (b ? t₁ | t₂) T₁
 
 notation Γ " ⊢ " t " : " T => has_type Γ t T
 
 theorem typing_example_1:
-  empty_ctx ⊢ ⦃Λ x:𝔹 ↦ x⦄ : ⦃𝔹 → 𝔹⦄ := has_type.abs (has_type.var rfl)
+  Γ₀ ⊢ ⦃Λ x:𝔹 ↦ x⦄ : ⦃𝔹 → 𝔹⦄ := has_type.abs (has_type.var rfl)
 
 /-
 ## Canonical forms
 -/
 
 theorem canonical_form_bool
-  (h₁: empty_ctx ⊢ t : 𝔹) (h₂: value t):
-  (t = ⊤) ∨ (t = ⊥) :=
+  (h₁: Γ₀ ⊢ t : 𝔹) (h₂: value t):
+  t = ⊤ ∨ t = ⊥ :=
   by cases h₁ <;> cases h₂ <;> simp
 
 theorem canonical_form_fun
-  (h₁: empty_ctx ⊢ t : (T₁ → T₂)) (h₂: value t):
+  (h₁: Γ₀ ⊢ t : (T₁ → T₂)) (h₂: value t):
   ∃x u, t = Λ x : T₁ ↦ u :=
   by cases h₁ <;> cases h₂; simp
 
@@ -41,53 +43,52 @@ theorem canonical_form_fun
 ## Progress
 -/
 
-theorem progress (h: empty_ctx ⊢ t : T):
-  value t ∨ ∃t', t ⇒ t' := by
-  {
-    generalize he: empty_ctx = Γ at h
-    induction h <;> cases he
-    . rename_i h; cases h
-    . exact Or.inl rfl
-    . simp at *
-      rename_i t₁ _ _ t₂ h₁ _ ih₁ ih₂
-      apply Or.inr
-      cases ih₁ with
-      | inl h =>
-        cases ih₂ with
-        | inl hh =>
-          have hc := canonical_form_fun h₁ h
-          cases hc with
-          | intro x hc =>
-            cases hc with
-            | intro w hc =>
-              rw [hc]
-              exists [x≔t₂]w
-              exact step.appabs hh
-        | inr hh =>
-          cases hh with
-          | intro w hh =>
-            exists t₁..w
-            exact step.app₂ h hh
-      | inr h =>
-        cases h with
-        | intro w h =>
-          exists (Term.app w t₂)
-          apply step.app₁ h
-    . exact Or.inl rfl
-    . exact Or.inl rfl
-    . simp at *
-      rename_i t₁ _ t₂ h₁ _ _ ih₁ _ _
-      cases ih₁ with
+theorem progress (h: Γ₀ ⊢ t : T): value t ∨ ∃w, t ⇒ w := by
+  generalize he: Γ₀ = Γ at h
+  induction h with
+  | abs => exact Or.inl rfl
+  | tt => exact Or.inl rfl
+  | ff => exact Or.inl rfl
+  | var h => cases he; cases h
+  | app t₁ t₂ h₁ _ ih₁ ih₂ =>
+    cases he
+    simp at *
+    apply Or.inr
+    cases ih₁ with
+    | inl h =>
+      cases ih₂ with
       | inl hh =>
-        apply Or.inr
-        have hc := canonical_form_bool h₁ hh
+        have hc := canonical_form_fun h₁ h
         cases hc with
-        | inl hc => exists t₁; rw [hc]; exact step.cond₁
-        | inr hc => exists t₂; rw [hc]; exact step.cond₂
+        | intro x hc =>
+          cases hc with
+          | intro w hc =>
+            rw [hc]
+            exists [x ≔ t₂]w
+            exact step.appabs hh
       | inr hh =>
-        apply Or.inr
         cases hh with
         | intro w hh =>
-          exists w ? t₁ | t₂
-          exact step.cond₃ hh
-  }
+          exists t₁..w
+          exact step.app₂ h hh
+    | inr h =>
+      cases h with
+      | intro w h =>
+        exists (Term.app w t₂)
+        apply step.app₁ h
+  | cond t₁ t₂ h₁ _ _ ih₁ =>
+    cases he
+    simp at *
+    cases ih₁ with
+    | inl hh =>
+      apply Or.inr
+      have hc := canonical_form_bool h₁ hh
+      cases hc with
+      | inl hc => exists t₁; rw [hc]; exact step.cond₁
+      | inr hc => exists t₂; rw [hc]; exact step.cond₂
+    | inr hh =>
+      apply Or.inr
+      cases hh with
+      | intro w hh =>
+        exists w ? t₁ | t₂
+        exact step.cond₃ hh
